This law implies that the cubing maps `B: x ↦ (x◇x)◇x` and `C: x ↦ x◇(x◇x)` are bijections that are inverses of each other and cube to the identity (namely `x = B(B(B(x))) = C(C(C(x))) = B(C(x)) = C(B(x))`), that right multiplications square to constant maps (namely `(y ◇ x) ◇ x` is `y`-independent, equal to `B(x)`), and that left multiplications square to `C` (and in particular are bijective).  The squaring map `S: x ↦ x◇x` cubes to the identity (`S(S(S(x)))=x`).  The left division operation defined by `x ◇ (x : y) = y` obeys the same law, `x = y : (y : ((z : x) : x))`.
