This law is a twist of the [involutive left multiplication law 16](https://teorth.github.io/equational_theories/implications/?16) `x = y◇(y◇x)` by the squaring map `S: x ↦ x◇x` and is equivalent to it if `S` is surjective.

In quasigroups (more generally when left multiplications are injective), this law is equivalent to [law 8](https://teorth.github.io/equational_theories/implications/?8) `x = x◇(x◇x)` together with [law 436](https://teorth.github.io/equational_theories/implications/?436) `x = x◇(y◇(y◇(x◇x)))`.
