This law is equivalent to the conjunction of [law 375](https://teorth.github.io/equational_theories/implications/?375) `x ◇ y = (x ◇ x) ◇ y` and the ["right-zero product" law 343](https://teorth.github.io/equational_theories/implications/?343) `x ◇ y = z ◇ (x ◇ y)` which states that all products are right zeros.

The free magma on some set `S` of generators for this law consists of finite non-empty lists of elements of `S`, with the operation `[s, …, t] ◇ [u, …, v] = [u, …, v]` when the second operand has more than one item, and `[s, s] ◇ [u] = [s, u]`, and otherwise `[s, …, t] ◇ [u] = [s, …, t, u]`.
