This law implies that the cubing maps `B: x ↦ (x◇x)◇x` and `C: x ↦ x◇(x◇x)` are bijections that are inverses of each other and cube to the identity (namely `x = B(B(B(x))) = C(C(C(x))) = B(C(x)) = C(B(x))`), that right multiplications square to constant maps (namely `(y◇x)◇x` is `y`-independent, equal to `B(x)`), and that left multiplications square to `C` (and in particular are bijective).  The squaring map `S: x ↦ x◇x` obeys `S(S(x)) = B(S(x))` hence `S(S(S(S(x))))=S(x)`.

This law is equivalent to [law 723](https://teorth.github.io/equational_theories/implications/?723) together with [law 3897](https://teorth.github.io/equational_theories/implications/?3897).

The left division operation defined by `x ◇ (x : y) = y` obeys law 42146, `y : (x : (y : (z : x))) = z : x`.
