This law implies the [associative law 4512](https://teorth.github.io/equational_theories/implications/?4512) and the [law 4362](https://teorth.github.io/equational_theories/implications/?4362) `xâ—‡(yâ—‡z) = yâ—‡(xâ—‡z)` dual to the non-associative-permutative law.  The squaring map `S: x â†¦ xâ—‡x` is idempotent, namely `S(S(x)) = S(x)`.

Its commutative version is [law 3385](https://teorth.github.io/equational_theories/implications/?3385).

The free magma on some set `S` of generators for this law is `S âŠ” (ğ’«(S) Ã— S)` where `ğ’«(S)` is the set of finite subsets of `S`, with the magma operation `sâ—‡t=({s},t)`, `(A,s)â—‡t=(Aâˆ†{s},t)`, `sâ—‡(B,t)=({s}âˆ†B,t)`, and `(A,s)â—‡(B,t)=(Aâˆ†{s}âˆ†B,t)` where `âˆ†` is the symmetric difference.  In particular, `sâ—‡sâ—‡t = (âˆ…,t)`.
