\chapter{Equation 906}\label{906-chapter}

In this chapter we study finite magmas that obey equation 906,
\begin{equation}\label{906}
  x = y \op ((y \op x) \op (x \op x))
\end{equation}
for all $x,y$.  We can write this as
\begin{equation}\label{906-a}
  L_y (L_y x \op Sx) = x.
\end{equation}
This implies that $L_y$ is surjective, hence invertible by finiteness, so
\begin{equation}\label{906-b}
   L_y x \op Sx = L_y^{-1} x.
\end{equation}
One corollary of this is that
$$ L_y x = L_z x \implies L_y^{-1} x = L_z^{-1} x.$$
By induction this implies
$$ L_y x = L_z x \implies L_y^{-n} x = L_z^{-n} x$$
for any $n \geq 1$.  Setting $n = N-2$ for $N>2$ a common period of $L_y,L_z$ (which exists by finiteness) we conclude that
\begin{equation}\label{lyzx}
  L_y x = L_z x \implies L_y^2 x = L_z^2 x.
\end{equation}

To use this, observe from \eqref{906-a} that
$$ L_x S^2 x = L_x (L_x x \op Sx) = x$$
while from \eqref{906-b} we have
$$ L_{L_x Sx} S^2 x = L_x Sx \op S S x = L_x^{-1} Sx = x.$$
Thus
$$ L_x S^2 x = L_{L_x Sx} S^2 x = x$$
and hence by \eqref{lyzx}
$$ L_x x = L_{L_x Sx} x$$
giving equation 3862,
\begin{equation}\label{3862}
  (x \op (x \op x)) \op x = x \op x.
\end{equation}
